lean/disaster-recovery/DisasterRecovery/Model/GlobalHelper.lean
@@ -1,0 +1,12 @@
+import DisasterRecovery.Model.Local
+
+namespace DisasterRecovery.Model.GlobalHelper
+
+open Local
+
+def receive (source : Location) : Message -> Event
+  | .gossip txid => .receiveGossip source txid .accepted
+  | .vote => .receiveVote source .accepted
+  | .iAmOpen => .receiveIAmOpen source .accepted
+
+end DisasterRecovery.Model.GlobalHelper
